CodeGen.v
@@ -1,0 +1,44 @@
+Require Import String.
+
+Require Import ZArith.
+Require Import List.
+Require Import Bool.
+Require Import Psatz.
+
+Require Import Linalg.
+Require Import Loop.
+Require Import PolyLang.
+
+Open Scope Z_scope.
+Open Scope list_scope.
+
+Parameter instr : Type.
+Parameter mem : Type.
+Parameter instr_semantics : instr -> list Z -> mem -> mem -> Prop.
+
+Inductive result (A : Type) :=
+| Ok : A -> result A
+| Err : string -> result A.
+
+Arguments Ok {A}.
+Arguments Err {A}.
+
+(* TODO *)
+Parameter split_polys : list polyhedron -> result (list (polyhedron * list nat)%type).
+
+Definition poly_disjoint pol1 pol2 := forall p, in_poly p pol1 = false \/ in_poly p pol2 = false.
+
+Fixpoint all_disjoint (l : list polyhedron) :=
+  match l with
+  | nil => True
+  | p :: l => (forall p2, In p2 l -> poly_disjoint p p2) /\ all_disjoint l
+  end.
+
+Axiom split_poly_disjoint :
+  forall pl r, split_polys pl = Ok r -> all_disjoint (map fst r).
+
+Axiom split_poly_indices :
+  forall pl r p l n, split_polys pl = Ok r -> In (p, l) r -> In n l -> (n < length pl)%nat.
+
+Axiom split_poly_eq :
+  forall pl r n p, split_polys pl = Ok r -> (n < length pl)%nat -> in_poly p (nth n pl nil) = existsb (fun z => in_poly p (fst z) && existsb (fun m => (m =? n)%nat) (snd z)) r.
